Carrier/SKAT_Term.thy
@@ -12,8 +12,7 @@ class ranked_alphabet =
   and rels :: "'a set"
   and NULL :: 'a
   and output_vars :: "'a itself \<Rightarrow> nat set"
-  assumes symbols_finite: "finite UNIV"
-  and funs_rels_disjoint: "funs \<inter> rels = {}"
+  assumes funs_rels_disjoint: "funs \<inter> rels = {}"
   and funs_rels_union: "funs \<union> rels = UNIV"
   and funs_exist: "funs \<noteq> {}"
   and rels_exist: "rels \<noteq> {}"
@@ -47,41 +46,41 @@ fun trm_subst :: "nat \<Rightarrow> 'a trm \<Rightarrow> 'a trm \<Rightarrow> 'a
   "trm_subst v s (Var v') = (if v' = v then s else Var v')"
 | "trm_subst v s (App f xs) = App f (map (trm_subst v s) xs)"
 
-inductive_set trms :: "'a::ranked_alphabet trm set" where
-  var: "Var n \<in> trms"
-| func: "\<lbrakk>f \<in> funs; arity f = n; xs \<in> lists trms; length xs = n\<rbrakk> \<Longrightarrow> App f xs \<in> trms"
+inductive_set wf_trms :: "'a::ranked_alphabet trm set" where
+  var: "Var n \<in> wf_trms"
+| func: "\<lbrakk>f \<in> funs; arity f = n; xs \<in> lists wf_trms; length xs = n\<rbrakk> \<Longrightarrow> App f xs \<in> wf_trms"
 
-lemma trm_subterms: "App f xs \<in> trms \<Longrightarrow> xs \<in> lists trms"
-  by (metis trm.simps(1) trm.simps(4) trms.simps)
+lemma trm_subterms: "App f xs \<in> wf_trms \<Longrightarrow> xs \<in> lists wf_trms"
+  by (metis (lifting) trm.simps(1) trm.simps(4) wf_trms.simps)
 
-lemma trm_subterms_var: "App f xs \<in> trms \<Longrightarrow> set xs \<subseteq> trms"
+lemma trm_subterms_var: "App f xs \<in> wf_trms \<Longrightarrow> set xs \<subseteq> wf_trms"
   by (metis in_lists_conv_set subset_code(1) trm_subterms)
 
 lemma map_in_lists: "map f xs \<in> lists X \<longleftrightarrow> f ` set xs \<subseteq> X"
   by (metis in_lists_conv_set in_mono set_map subsetI)
 
-lemma trm_subst_wf: "\<lbrakk>s \<in> trms; x \<in> trms\<rbrakk> \<Longrightarrow> trm_subst v s x \<in> trms"
-proof (rule trms.induct[of x "\<lambda>x. trm_subst v s x \<in> trms"], safe)
-  fix n assume "s \<in> trms" and "x \<in> trms" thus "trm_subst v s (Var n) \<in> trms"
-    by (metis trm_subst.simps(1) trms.var)
+lemma trm_subst_wf: "\<lbrakk>s \<in> wf_trms; x \<in> wf_trms\<rbrakk> \<Longrightarrow> trm_subst v s x \<in> wf_trms"
+proof (rule wf_trms.induct[of x "\<lambda>x. trm_subst v s x \<in> wf_trms"], safe)
+  fix n assume "s \<in> wf_trms" and "x \<in> wf_trms" thus "trm_subst v s (Var n) \<in> wf_trms"
+    by (metis trm_subst.simps(1) wf_trms.var)
 next
   fix f :: "'a::ranked_alphabet" and xs :: "'a trm list"
-  assume s_trm: "s \<in> trms" and x_trm: "x \<in> trms" and f_fun: "f \<in> funs"
+  assume s_trm: "s \<in> wf_trms" and x_trm: "x \<in> wf_trms" and f_fun: "f \<in> funs"
   and xs_len: "length xs = arity f"
-  and ind_hyp: "\<forall>x\<in>set xs. x \<in> trms \<inter> {x. trm_subst v s x \<in> trms}"
-  show "trm_subst v s (App f xs) \<in> trms"
-  proof (simp, rule trms.func[of _ "length xs"])
+  and ind_hyp: "\<forall>x\<in>set xs. x \<in> wf_trms \<inter> {x. trm_subst v s x \<in> wf_trms}"
+  show "trm_subst v s (App f xs) \<in> wf_trms"
+  proof (simp, rule wf_trms.func[of _ "length xs"])
     show "f \<in> funs" using f_fun .
     show "arity f = length xs" by (simp add: xs_len)
-    show "map (trm_subst v s) xs \<in> lists trms"
+    show "map (trm_subst v s) xs \<in> lists wf_trms"
       by (simp add: map_in_lists image_def, auto, metis Int_Collect ind_hyp)
     show "length (map (trm_subst v s) xs) = length xs"
       by (metis length_map)
   qed
 qed
 
-lemma trms_const: "\<lbrakk>f \<in> funs; arity f = 0\<rbrakk> \<Longrightarrow> App f [] \<in> trms"
-  by (rule trms.func, simp_all add: lists_def)
+lemma wf_trms_const: "\<lbrakk>f \<in> funs; arity f = 0\<rbrakk> \<Longrightarrow> App f [] \<in> wf_trms"
+  by (rule wf_trms.func, simp_all add: lists_def)
 
 (* +------------------------------------------------------------------------+ *)
 subsection {* n-tuples *}
@@ -125,235 +124,296 @@ record ('a, 'b) interp = "'b partial_object" +
   mf :: "'a \<Rightarrow> 'b list \<Rightarrow> 'b"
   mr :: "'a \<Rightarrow> 'b relation"
 
-locale valid_interp =
-  fixes D :: "('a::ranked_alphabet, 'b) interp"
-  assumes fun_meaning: "f \<in> funs \<Longrightarrow> mf D f : (carrier D)\<^bsup>arity f\<^esup> \<rightarrow> carrier D"
-  and rel_meaning: "P \<in> rels \<Longrightarrow> mr D P \<subseteq> (carrier D)\<^bsup>arity P\<^esup>"
-
 type_synonym 'a mem = "nat \<Rightarrow> 'a"
 
 fun eval_trm :: "('a::ranked_alphabet, 'b) interp \<Rightarrow> (nat \<Rightarrow> 'b) \<Rightarrow> 'a trm \<Rightarrow> 'b" where
   "eval_trm D mem (Var n) = mem n"
 | "eval_trm D mem (App f xs) = mf D f (map (eval_trm D mem) xs)"
 
-lemma eval_trm_closed:
-  assumes valid_ip: "valid_interp D"
-  and valid_mem: "\<forall>n. mem n \<in> carrier D"
-  and trms: "x \<in> trms" shows "eval_trm D mem x \<in> carrier D"
-  using trms
-proof (induct x)
-  fix n
-  show "eval_trm D mem (Var n) \<in> carrier D"
-    by (simp add: eval_trm.simps, metis valid_mem)
-next
-  fix f :: "'b::ranked_alphabet" and n xs
-  assume f_funs: "f \<in> funs" and f_arity: "arity f = n"
-  and xs_eval: "xs \<in> lists (trms \<inter> {x. eval_trm D mem x \<in> carrier D})"
-  and xs_len: "length xs = n"
+definition null :: "'a::ranked_alphabet trm" where
+  "null \<equiv> App NULL []"
 
-  have "xs \<in> lists {x. eval_trm D mem x \<in> carrier D}"
-    by (metis (lifting) xs_eval IntD2 lists_Int_eq)
-  hence "set xs \<subseteq> {x. eval_trm D mem x \<in> carrier D}"
-    by (metis lists_eq_set mem_Collect_eq)
-
-  hence "map (eval_trm D mem) xs \<in> carrier D\<^bsup>length xs\<^esup>"
-    by (induct xs, simp_all add: map_def)
-
-  hence "mf D f (map (eval_trm D mem) xs) \<in> carrier D"
-    apply (rule typed_application)
-    apply (simp add: xs_len f_arity[symmetric])
-    by (rule valid_interp.fun_meaning[OF valid_ip f_funs])
-
-  thus "eval_trm D mem (App f xs) \<in> carrier D"
-    by (simp add: eval_trm.simps(1))
-qed
-
-typedef (open) 'a wf_trm = "trms::'a::ranked_alphabet trm set"
-  by (rule_tac x = "Var 0" in exI, rule trms.var)
-
-definition var :: "nat \<Rightarrow> 'a::ranked_alphabet wf_trm" where
-  "var i \<equiv> Abs_wf_trm (Var i)"
-
-lemma Rep_var [simp]: "Rep_wf_trm (var n) = Var n"
-  by (metis Abs_wf_trm_inverse trms.var var_def)
-
-lemma Abs_var [simp]: "Abs_wf_trm (Var n) = var n"
-  by (metis var_def)
-
-definition null :: "'a::ranked_alphabet wf_trm" where
-  "null \<equiv> Abs_wf_trm (App NULL [])"
-
-definition wf_trm_vars :: "'a::ranked_alphabet wf_trm \<Rightarrow> nat set" where
-  "wf_trm_vars x = trm_vars (Rep_wf_trm x)"
-
-definition eval_wf_trm :: "('a::ranked_alphabet, 'b) interp \<Rightarrow> (nat \<Rightarrow> 'b) \<Rightarrow> 'a wf_trm \<Rightarrow> 'b" where
-  "eval_wf_trm D mem x \<equiv> eval_trm D mem (Rep_wf_trm x)"
-
-lemma eval_wf_trm_closed:
-  assumes valid_ip: "valid_interp D"
-  and valid_mem: "\<forall>n. mem n \<in> carrier D"
-  shows "eval_wf_trm D mem x \<in> carrier D"
-  by (metis Rep_wf_trm eval_trm_closed eval_wf_trm_def valid_ip valid_mem)
-
-definition wf_trm_subst :: "nat \<Rightarrow> 'a::ranked_alphabet wf_trm \<Rightarrow> 'a wf_trm \<Rightarrow> 'a wf_trm" where
-  "wf_trm_subst v s x \<equiv> Abs_wf_trm (trm_subst v (Rep_wf_trm s) (Rep_wf_trm x))"
-
-abbreviation wf_trm_subst_notation :: "'a::ranked_alphabet wf_trm \<Rightarrow> nat \<Rightarrow> 'a wf_trm \<Rightarrow> 'a wf_trm"
+abbreviation trm_subst_notation :: "'a::ranked_alphabet trm \<Rightarrow> nat \<Rightarrow> 'a trm \<Rightarrow> 'a trm"
   ("_[_|_]" [100,100,100] 101) where
-  "s[x|t] \<equiv> wf_trm_subst x t s"
+  "s[x|t] \<equiv> trm_subst x t s"
 
 (* +------------------------------------------------------------------------+ *)
 subsection {* Predicates *}
 (* +------------------------------------------------------------------------+ *)
 
-datatype 'a pred = Pred 'a "'a wf_trm list"
+datatype 'a pred = Pred 'a "'a trm list"
 
-inductive_set preds :: "'a::ranked_alphabet pred set" where
-  "\<lbrakk>P \<in> rels; arity P = length xs\<rbrakk> \<Longrightarrow> Pred P xs \<in> preds"
+inductive_set wf_preds :: "'a::ranked_alphabet pred set" where
+  "\<lbrakk>P \<in> rels; arity P = length xs\<rbrakk> \<Longrightarrow> Pred P xs \<in> wf_preds"
 
 primrec eval_pred :: "('a::ranked_alphabet, 'b) interp \<Rightarrow> 'b mem \<Rightarrow> 'a pred \<Rightarrow> bool" where
-  "eval_pred D mem (Pred P xs) \<longleftrightarrow> map (eval_wf_trm D mem) xs \<in> mr D P"
+  "eval_pred D mem (Pred P xs) \<longleftrightarrow> map (eval_trm D mem) xs \<in> mr D P"
 
-primrec pred_subst :: "nat \<Rightarrow> 'a::ranked_alphabet wf_trm \<Rightarrow> 'a pred \<Rightarrow> 'a pred" where
-  "pred_subst v s (Pred P xs) = Pred P (map (wf_trm_subst v s) xs)"
-
-typedef (open) 'a wf_pred = "preds::'a::ranked_alphabet pred set"
-  by (metis Ex_list_of_length equals0I preds.intros rels_exist)
-
-definition eval_wf_pred :: "('a::ranked_alphabet, 'b) interp \<Rightarrow> 'b mem \<Rightarrow> 'a wf_pred \<Rightarrow> bool" where
-  "eval_wf_pred D mem P \<equiv> eval_pred D mem (Rep_wf_pred P)"
-
-definition
-  wf_pred_subst :: "nat \<Rightarrow> 'a::ranked_alphabet wf_trm \<Rightarrow> 'a wf_pred \<Rightarrow> 'a wf_pred"
-  where
-  "wf_pred_subst v s \<equiv> Abs_wf_pred \<circ> pred_subst v s \<circ> Rep_wf_pred"
+primrec pred_subst :: "nat \<Rightarrow> 'a::ranked_alphabet trm \<Rightarrow> 'a pred \<Rightarrow> 'a pred" where
+  "pred_subst v s (Pred P xs) = Pred P (map (trm_subst v s) xs)"
 
 abbreviation
-  wf_pred_subst_notation :: "'a::ranked_alphabet wf_pred \<Rightarrow> nat \<Rightarrow> 'a wf_trm \<Rightarrow> 'a wf_pred"
+  pred_subst_notation :: "'a::ranked_alphabet pred \<Rightarrow> nat \<Rightarrow> 'a trm \<Rightarrow> 'a pred"
   ("_[_|_]" [100,100,100] 101) where
-  "s[x|t] \<equiv> wf_pred_subst x t s"
+  "s[x|t] \<equiv> pred_subst x t s"
 
 (* Simple while programs *)
 
-datatype 'a prog = If "'a wf_pred" "'a prog" "'a prog"
-                 | While "'a wf_pred" "'a prog"
-                 | Seq "'a prog list"
-                 | Assign nat "'a wf_trm"
+datatype 'a prog = If "'a pred" "'a prog" "'a prog"
+                 | While "'a pred" "'a prog"
+                 | Seq "'a prog" "'a prog"
+                 | Assign nat "'a trm"
+                 | Skip
+
+fun prog_preds :: "'a prog \<Rightarrow> 'a pred set" where
+  "prog_preds (If P x y) = {P} \<union> prog_preds x \<union> prog_preds y"
+| "prog_preds (While P x) = {P} \<union> prog_preds x"
+| "prog_preds (Seq x y) = prog_preds x \<union> prog_preds y"
+| "prog_preds (Assign _ _) = {}"
+| "prog_preds Skip = {}"
+
+fun prog_whiles :: "'a prog \<Rightarrow> 'a prog set" where
+  "prog_whiles (If P x y) = prog_whiles x \<union> prog_whiles y"
+| "prog_whiles (While P x) = {While P x} \<union> prog_whiles x"
+| "prog_whiles (Seq x y) = prog_whiles x \<union> prog_whiles y"
+| "prog_whiles (Assign _ _) = {}"
+| "prog_whiles Skip = {}"
 
 fun eval_prog :: "nat \<Rightarrow> ('a::ranked_alphabet, 'b) interp \<Rightarrow> 'b mem \<Rightarrow> 'a prog \<Rightarrow> 'b mem option" where
   "eval_prog 0 _ _ _ = None"
 | "eval_prog (Suc n) D mem (If P x y) =
-     (if eval_wf_pred D mem P
+     (if eval_pred D mem P
      then eval_prog n D mem x
      else eval_prog n D mem y)"
 | "eval_prog (Suc n) D mem (While P x) =
-     (if eval_wf_pred D mem P
+     (if eval_pred D mem P
      then case eval_prog n D mem x of
        Some mem' \<Rightarrow> eval_prog n D mem' (While P x)
      | None \<Rightarrow> None
      else Some mem)"
-| "eval_prog (Suc n) D mem (Seq (x#xs)) =
+| "eval_prog (Suc n) D mem (Seq x y) =
      (case eval_prog n D mem x of
-       Some mem' \<Rightarrow> eval_prog n D mem (Seq xs)
+       Some mem' \<Rightarrow> eval_prog n D mem' y
      | None \<Rightarrow> None)"
-| "eval_prog (Suc n) D mem (Seq []) = Some mem"
+| "eval_prog (Suc n) D mem Skip = Some mem"
 | "eval_prog (Suc n) D mem (Assign m x) =
-     (Some (\<lambda>v. if v = m then eval_wf_trm D mem x else mem v))"
+     (Some (\<lambda>v. if v = m then eval_trm D mem x else mem v))"
 
-definition terminates :: "'a::ranked_alphabet prog \<Rightarrow> bool" where
-  "terminates prgm \<equiv> \<exists>steps. \<forall>D mem. valid_interp D \<longrightarrow> eval_prog steps D mem prgm \<noteq> None"
+(*
+lemma min_terminates: "eval_prog n D mem pgm = Some r \<Longrightarrow> eval_prog (n + m) D mem pgm = Some r"
+  sorry
 
-definition tprogs :: "'a::ranked_alphabet prog set" where
-  "tprogs \<equiv> {prgm. terminates TYPE('b) prgm}"
+definition terminates :: "('a::ranked_alphabet, 'b) interp \<Rightarrow> 'a prog \<Rightarrow> bool" where
+  "terminates D prgm \<equiv> \<exists>steps. \<forall>mem. eval_prog steps D mem prgm \<noteq> None"
 
-fun FV' :: "'a trm \<Rightarrow> nat set" where
-  "FV' (Var v) = {v}"
-| "FV' (App f xs) = foldr op \<union> (map FV' xs) {}"
+lemma Skip_terminates [intro!]: "terminates D Skip"
+  by (simp add: terminates_def, rule_tac x = 1 in exI, auto)
 
-definition FV :: "'a::ranked_alphabet wf_trm \<Rightarrow> nat set" where
-  "FV \<equiv> FV' \<circ> Rep_wf_trm"
+lemma Assign_terminates [intro!]: "terminates D (Assign x s)"
+  by (simp add: terminates_def, rule_tac x = 1 in exI, auto)
 
-lemma FV_is_FV': "x \<in> trms \<Longrightarrow> FV (Abs_wf_trm x) = FV' x"
-  by (metis Abs_wf_trm_inverse FV_def o_apply)
+lemma If_terminates [intro]: "\<lbrakk>terminates D x; terminates D y\<rbrakk> \<Longrightarrow> terminates D (If P x y)"
+proof (simp add: terminates_def)
+  assume "\<exists>steps. \<forall>mem. \<exists>r. eval_prog steps D mem x = Some r"
+  and "\<exists>steps. \<forall>mem. \<exists>r. eval_prog steps D mem y = Some r"
 
-lemma app_FV': "v \<notin> FV' (App f xs) \<Longrightarrow> \<forall>x\<in>set xs. v \<notin> FV' x"
+  then obtain x_steps and y_steps
+    where "\<forall>mem. \<exists>r. eval_prog x_steps D mem x = Some r"
+    and "\<forall>mem. \<exists>r. eval_prog y_steps D mem y = Some r"
+    by auto
+
+  thus "\<exists>steps. \<forall>mem. \<exists>r. eval_prog steps D mem (If P x y) = Some r"
+    apply (rule_tac x = "Suc (max x_steps y_steps)" in exI)
+    apply auto
+    apply (cases "x_steps > y_steps")
+    apply smt
+    apply (subgoal_tac "\<exists>n. max x_steps y_steps = x_steps + n")
+    apply (metis min_terminates)
+    apply (metis add_0_right le_iff_add less_imp_add_positive linorder_cases max_absorb2)
+    apply (cases "y_steps > x_steps")
+    apply smt
+    apply (subgoal_tac "\<exists>n. max x_steps y_steps = y_steps + n")
+    apply (metis min_terminates)
+    by (metis add_0_right le_iff_add less_imp_add_positive linorder_cases max_absorb2 min_max.sup.commute)
+qed
+
+lemma Seq_terminates [intro]: "\<lbrakk>terminates D x; terminates D y\<rbrakk> \<Longrightarrow> terminates D (Seq x y)"
+proof (simp add: terminates_def)
+  assume "\<exists>steps. \<forall>mem. \<exists>r. eval_prog steps D mem x = Some r"
+  and "\<exists>steps. \<forall>mem. \<exists>r. eval_prog steps D mem y = Some r"
+
+  then obtain x_steps and y_steps
+    where "\<forall>mem. \<exists>r. eval_prog x_steps D mem x = Some r"
+    and "\<forall>mem. \<exists>r. eval_prog y_steps D mem y = Some r"
+    by auto
+
+  thus "\<exists>steps. \<forall>mem. \<exists>r. eval_prog steps D mem (Seq x y) = Some r"
+    apply (rule_tac x = "Suc (x_steps + y_steps)" in exI, simp)
+    by (metis (lifting) min_terminates nat_add_commute option.simps(5))
+qed
+
+lemma Seq_sub_terminates: assumes "terminates D (Seq x y)" shows "terminates D x" and "terminates D y"
+proof (insert assms)
+  assume "terminates D (Seq x y)"
+  then obtain n where seq_term: "\<forall>mem. eval_prog (Suc n) D mem (Seq x y) \<noteq> None"
+    by (metis eval_prog.simps(1) not0_implies_Suc terminates_def)
+  hence x_term: "\<forall>mem. eval_prog n D mem x \<noteq> None"
+    by (auto, metis not_Some_eq option.simps(4))
+  thus "terminates D x"
+    by (metis terminates_def)
+  from this and assms obtain m where "\<forall>mem. eval_prog (Suc (Suc m)) D mem (Seq x y) \<noteq> None"
+    by (simp add: terminates_def, metis add_Suc_right eval_prog.simps(4) min_terminates)
+  from this and x_term have "\<forall>mem. eval_prog n D mem y \<noteq> None"
+    sorry
+  thus "terminates D y"
+    by (metis terminates_def)
+qed
+
+(*
+lemma least_steps: "terminates D x \<Longrightarrow> \<exists>!n. eval_prog n D mem x \<noteq> None \<and> eval_prog (n - 1) D mem x = None"
+proof (induct x)
+  assume "terminates D Skip"
+  hence "\<exists>n. eval_prog n D mem Skip \<noteq> None \<and> eval_prog (n - 1) D mem Skip = None"
+    by (rule_tac x = 1 in exI, auto)
+  thus "\<exists>!n. eval_prog n D mem Skip \<noteq> None \<and> eval_prog (n - 1) D mem Skip = None"
+    by (auto, metis diff_Suc_less diffs0_imp_equal eval_prog.simps(5) less_Suc0 nat.exhaust option.simps(3))
+next
+  fix x s
+  assume "terminates D (Assign x s)"
+  hence "eval_prog 1 D mem (Assign x s) \<noteq> None \<and> eval_prog 0 D mem (Assign x s) = None"
+    by auto
+  moreover
+  {
+    fix n :: nat
+    assume "n > 1"
+    then obtain m where n_def: "n = Suc (Suc m)"
+      by (metis One_nat_def gr_implies_not0 linorder_not_le nat.exhaust order_refl)
+    hence "eval_prog (Suc (Suc m)) D mem (Assign x s) \<noteq> None \<and> eval_prog (Suc m) D mem (Assign x s) \<noteq> None"
+      by auto
+    hence "eval_prog n D mem (Assign x s) \<noteq> None \<and> eval_prog (n - 1) D mem (Assign x s) \<noteq> None"
+      by (metis diff_Suc_1 n_def)
+  }
+  ultimately show "\<exists>!n. eval_prog n D mem (Assign x s) \<noteq> None \<and> eval_prog (n - 1) D mem (Assign x s) = None"
+    by smt
+next
+  fix x1 x2
+  assume ind_hyp1: "terminates D x1 \<Longrightarrow> \<exists>!n. eval_prog n D mem x1 \<noteq> None \<and> eval_prog (n - 1) D mem x1 = None"
+  and ind_hyp2: "terminates D x2 \<Longrightarrow> \<exists>!n. eval_prog n D mem x2 \<noteq> None \<and> eval_prog (n - 1) D mem x2 = None"
+  and "terminates D (Seq x1 x2)"
+  hence "\<exists>!n. eval_prog n D mem x1 \<noteq> None \<and> eval_prog (n - 1) D mem x1 = None"
+  and "\<exists>!n. eval_prog n D mem x2 \<noteq> None \<and> eval_prog (n - 1) D mem x2 = None"
+    
+
+definition steps_eq :: "('a::ranked_alphabet, 'b) interp \<Rightarrow> nat \<Rightarrow> 'b mem \<Rightarrow> 'a prog \<Rightarrow> 'a prog \<Rightarrow> bool" where
+  "steps_eq D n mem pgm1 pgm2 \<equiv> eval_prog n D mem pgm1 = eval_prog n D mem pgm2"
+
+definition schematic_eq :: "('a::ranked_alphabet, 'b) interp \<Rightarrow> 'a prog \<Rightarrow> 'a prog \<Rightarrow> bool" where
+  "schematic_eq D pgm1 pgm2 \<equiv> \<forall>mem. \<exists>n. steps_eq D n mem pgm1 pgm2 \<and> eval_prog n D mem pgm1 \<noteq> None"
+
+lemma schematic_eq_var: "schematic_eq D pgm1 pgm2 = (\<exists>n. \<forall>mem. steps_eq D n mem pgm1 pgm2 \<and> eval_prog n D mem pgm1 \<noteq> None)"
+proof
+  assume "schematic_eq D pgm1 pgm2"
+  then obtain m where "m = Max {n. steps_eq D n mem pgm1 pgm2
+
+lemma schematic_eq_var: "schematic_eq D pgm1 pgm2 = (\<forall>mem. (\<exists>n. (eval_prog n D mem pgm1 = eval_prog n D mem pgm2) \<and> (eval_prog n D mem pgm1 \<noteq> None)))"
+  apply (simp add: schematic_eq_def, auto, blast)
+  apply (rule_tac x = "Max {n. eval_prog n D mem pgm1 = eval_prog n D mem pgm2 \<and> eval_prog n D mem pgm1 \<noteq> None}" in exI)
+  apply auto
+
+lemma If_subterm_1: "\<lbrakk>terminates D (If P x y); \<forall>mem. eval_wf_pred D mem P\<rbrakk> \<Longrightarrow> schematic_eq D (If P x y) x"
+proof (simp add: schematic_eq_def)
+  assume "terminates D (If P x y)" and "\<forall>mem. eval_wf_pred D mem P"
+  then moreover obtain m where "\<forall>mem. eval_prog m D mem (If P x y) \<noteq> None"
+    by (metis terminates_def)
+  ultimately have "\<exists>n. \<forall>mem. eval_prog n D mem (If P x y) = eval_prog n D mem x \<and>
+                             (\<exists>r. eval_prog n D mem (If P x y) = Some r)"
+    apply (rule_tac x = "Suc m" in exI, auto)
+    apply (metis Nat.add_0_right add_Suc_right eval_prog.simps(2) min_terminates)
+    by (metis add.comm_neutral add_Suc_right eval_prog.simps(2) min_terminates)
+  thus "(\<exists>n. \<forall>mem. eval_prog n D mem (prog.If P x y) =
+                   eval_prog n D mem x \<and>
+                   (\<exists>ya. eval_prog n D mem (prog.If P x y) = Some ya)) \<or>
+        (\<forall>n mem. eval_prog n D mem (prog.If P x y) = eval_prog n D mem x)"
+    by metis
+qed
+
+lemma If_subterm_2: "\<lbrakk>terminates D (If P x y); \<forall>mem. \<not> eval_wf_pred D mem P\<rbrakk> \<Longrightarrow> schematic_eq D (If P x y) y"
+proof (simp add: schematic_eq_def)
+  assume "terminates D (If P x y)" and "\<forall>mem. \<not> eval_wf_pred D mem P"
+  then moreover obtain m where "\<forall>mem. eval_prog m D mem (If P x y) \<noteq> None"
+    by (metis terminates_def)
+  ultimately show "\<exists>n. \<forall>mem. eval_prog n D mem (If P x y) = eval_prog n D mem y \<and>
+                             (\<exists>r. eval_prog n D mem (If P x y) = Some r)"
+    apply (rule_tac x = "Suc m" in exI, auto)
+    apply (metis Nat.add_0_right add_Suc_right eval_prog.simps(2) min_terminates)
+    by (metis add.comm_neutral add_Suc_right eval_prog.simps(2) min_terminates)
+qed
+
+lemma same_program_comm: "same_program D pgm1 pgm2 \<Longrightarrow> same_program D pgm2 pgm1"
+  by (auto simp add: same_program_def, metis)
+
+lemma same_program_trans: "\<lbrakk>same_program D pgm1 pgm2; same_program D pgm2 pgm3\<rbrakk> \<Longrightarrow> same_program D pgm1 pgm3"
+  apply (auto simp add: same_program_def)
+  by (metis comm_semiring_1_class.normalizing_semiring_rules(24) min_terminates)
+
+lemma same_program_refl: "terminates D pgm \<Longrightarrow> same_program D pgm pgm"
+  by (auto simp add: same_program_def terminates_def)
+
+lemma all_loops_terminate: "\<lbrakk>\<And>loop. loop \<in> prog_whiles pgm \<Longrightarrow> terminates D loop\<rbrakk> \<Longrightarrow> terminates D pgm"
+  by (induct pgm, auto)
+
+lemma "terminates D pgm1 \<Longrightarrow> \<exists>pgm2. (\<forall>loop. loop \<in> prog_whiles pgm2 \<longrightarrow> terminates D loop) \<and> (same_result D pgm1 pgm2)"
+  apply (induct pgm1)
+
+*)
+*)
+
+fun FV :: "'a trm \<Rightarrow> nat set" where
+  "FV (Var v) = {v}"
+| "FV (App f xs) = foldr op \<union> (map FV xs) {}"
+
+lemma app_FV: "v \<notin> FV (App f xs) \<Longrightarrow> \<forall>x\<in>set xs. v \<notin> FV x"
   by (erule contrapos_pp, simp, induct xs, auto)
 
-lemma no_FV' [simp]: "v \<notin> FV' s \<Longrightarrow> trm_subst v t s = s"
+lemma no_FV [simp]: "v \<notin> FV s \<Longrightarrow> s[v|t] = s"
 proof (induct s)
   fix f xs
-  assume asm: "\<forall>x\<in>set xs. v \<notin> FV' x \<longrightarrow> trm_subst v t x = x"
-    and "v \<notin> FV' (App f xs)"
-  hence "\<forall>x\<in>set xs. v \<notin> FV' x"
-    by (metis app_FV')
+  assume asm: "\<forall>x\<in>set xs. v \<notin> FV x \<longrightarrow> trm_subst v t x = x"
+    and "v \<notin> FV (App f xs)"
+  hence "\<forall>x\<in>set xs. v \<notin> FV x"
+    by (metis app_FV)
   thus "trm_subst v t (App f xs) = App f xs"
     by (metis (lifting) asm map_idI trm_subst.simps(2))
 next
-  fix v' assume "v \<notin> FV' (Var v')"
+  fix v' assume "v \<notin> FV (Var v')"
   thus "trm_subst v t (Var v') = Var v'" by simp
 next
-  show "\<forall>x\<in>set []. v \<notin> FV' x \<longrightarrow> trm_subst v t x = x" by simp
+  show "\<forall>x\<in>set []. v \<notin> FV x \<longrightarrow> trm_subst v t x = x" by simp
 next
   fix x xs
-  assume "v \<notin> FV' x \<Longrightarrow> trm_subst v t x = x"
-    and "\<forall>y\<in>set xs. v \<notin> FV' y \<longrightarrow> trm_subst v t y = y"
-  thus "\<forall>y\<in>set (x # xs). v \<notin> FV' y \<longrightarrow> trm_subst v t y = y"
+  assume "v \<notin> FV x \<Longrightarrow> trm_subst v t x = x"
+    and "\<forall>y\<in>set xs. v \<notin> FV y \<longrightarrow> trm_subst v t y = y"
+  thus "\<forall>y\<in>set (x # xs). v \<notin> FV y \<longrightarrow> trm_subst v t y = y"
     by auto
 qed
-
-lemma no_FV [simp]: "v \<notin> FV s \<Longrightarrow> s[v|t] = s"
-  by (induct s, metis FV_def Rep_wf_trm_inverse no_FV' o_apply wf_trm_subst_def)
 
 primrec pred_vars :: "'a::ranked_alphabet pred \<Rightarrow> nat set" where
   "pred_vars (Pred P xs) = \<Union> (set (map FV xs))"
 
-lemma no_pred_vars: "v \<notin> pred_vars \<phi> \<Longrightarrow> pred_subst v t \<phi> = \<phi>"
+lemma no_pred_vars: "v \<notin> pred_vars \<phi> \<Longrightarrow> \<phi>[v|t] = \<phi>"
 proof (induct \<phi>, simp)
-  fix xs :: "'a wf_trm list" assume "\<forall>x\<in>set xs. v \<notin> FV x"
-  thus "map (wf_trm_subst v t) xs = xs"
+  fix xs :: "'a trm list" assume "\<forall>x\<in>set xs. v \<notin> FV x"
+  thus "map (trm_subst v t) xs = xs"
     by (induct xs, simp_all)
 qed
 
-definition wf_pred_vars :: "'a::ranked_alphabet wf_pred \<Rightarrow> nat set" where
-  "wf_pred_vars P = pred_vars (Rep_wf_pred P)"
-
-lemma no_wf_pred_vars [simp]: "v \<notin> wf_pred_vars \<phi> \<Longrightarrow> wf_pred_subst v t \<phi> = \<phi>"
-  apply (induct \<phi>)
-  by (metis Abs_wf_pred_inverse no_pred_vars o_eq_dest_lhs wf_pred_subst_def wf_pred_vars_def)
-
 ML {*
-
 structure AlphabetRules = Named_Thms
   (val name = @{binding "alphabet"}
    val description = "Alphabet rules")
-
-fun wf_trm_abs_inverse_tac simpset ctxt =
-  EqSubst.eqsubst_tac ctxt [0] @{thms Abs_wf_trm_inverse} 1
-  THEN REPEAT
-    (CHANGED (asm_full_simp_tac
-      (simpset addsimps @{thms FV_def} addsimps AlphabetRules.get ctxt) 1)
-    ORELSE resolve_tac @{thms trms.intros} 1)
-
-fun wf_pred_abs_inverse_tac simpset ctxt =
-  EqSubst.eqsubst_tac ctxt [0] @{thms Abs_wf_pred_inverse} 1
-  THEN REPEAT
-    (CHANGED (asm_full_simp_tac
-      (simpset addsimps @{thms wf_pred_vars_def} addsimps AlphabetRules.get ctxt) 1)
-    ORELSE resolve_tac @{thms preds.intros} 1
-    ORELSE rtac @{thm conjI} 1)
-
-fun wf_simp_tac simpset =
-  Subgoal.FOCUS (fn {context, ...} =>
-    REPEAT (wf_trm_abs_inverse_tac simpset context)
-    THEN REPEAT (wf_pred_abs_inverse_tac simpset context))
-
 *}
 
 setup {* AlphabetRules.setup *}
-
-method_setup wf_simp = {*
-Scan.succeed (fn ctxt => SIMPLE_METHOD' (wf_simp_tac (simpset_of ctxt) ctxt))
-*}
 
 lemma trm_simple_induct': "\<lbrakk>\<And>f xs. (\<forall>x\<in>set xs. P x) \<Longrightarrow> P (App f xs); \<And>n. P (Var n)\<rbrakk> \<Longrightarrow> P s \<and> (\<forall>x\<in>set []. P x)"
   by (rule trm.induct[of "\<lambda>xs. (\<forall>x\<in>set xs. P x)" P], simp_all)
@@ -361,19 +421,19 @@ lemma trm_simple_induct': "\<lbrakk>\<And>f xs. (\<forall>x\<in>set xs. P x) \<L
 lemma trm_simple_induct: "\<lbrakk>\<And>n. P (Var n); \<And>f xs. (\<forall>x\<in>set xs. P x) \<Longrightarrow> P (App f xs)\<rbrakk> \<Longrightarrow> P s"
   by (metis trm_simple_induct')
 
-lemma foldr_FV': "foldr op \<union> (map FV' xs) {} = \<Union> (FV' ` set xs)"
+lemma foldr_FV: "foldr op \<union> (map FV xs) {} = \<Union> (FV ` set xs)"
   by (induct xs, auto)
 
-lemma eval_trm_eq_mem: "(\<forall>v\<in>FV' s. m1 v = m2 v) \<Longrightarrow> eval_trm D m1 s = eval_trm D m2 s"
+lemma eval_trm_eq_mem: "(\<forall>v\<in>FV s. m1 v = m2 v) \<Longrightarrow> eval_trm D m1 s = eval_trm D m2 s"
 proof (induct rule: trm_simple_induct, auto)
   fix f :: "'a" and xs :: "'a trm list"
-  assume asm1: "\<forall>x\<in>set xs. (\<forall>v\<in>FV' x. m1 v = m2 v) \<longrightarrow> eval_trm D m1 x = eval_trm D m2 x"
-  and asm2: "\<forall>v\<in>foldr op \<union> (map FV' xs) {}. m1 v = m2 v"
-  have "foldr op \<union> (map FV' xs) {} = \<Union> (FV' ` set xs)"
+  assume asm1: "\<forall>x\<in>set xs. (\<forall>v\<in>FV x. m1 v = m2 v) \<longrightarrow> eval_trm D m1 x = eval_trm D m2 x"
+  and asm2: "\<forall>v\<in>foldr op \<union> (map FV xs) {}. m1 v = m2 v"
+  have "foldr op \<union> (map FV xs) {} = \<Union> (FV ` set xs)"
     by (induct xs, auto)
-  hence "\<forall>v\<in>\<Union>(FV' ` set xs). m1 v = m2 v"
+  hence "\<forall>v\<in>\<Union>(FV ` set xs). m1 v = m2 v"
     by (metis asm2)
-  hence "\<forall>x\<in>set xs. (\<forall>v\<in>FV' x. m1 v = m2 v)"
+  hence "\<forall>x\<in>set xs. (\<forall>v\<in>FV x. m1 v = m2 v)"
     by (metis UnionI imageI)
   hence "\<forall>x\<in>set xs. eval_trm D m1 x = eval_trm D m2 x"
     by (metis asm1)
@@ -395,16 +455,8 @@ definition halt_null :: "('a::ranked_alphabet, 'b) interp \<Rightarrow> 'b mem \
   where
   "halt_null D mem \<equiv> \<lambda>v. if v \<notin> output_vars TYPE('a) then mf D NULL [] else mem v"
 
-definition wf_assign ::
-  "('a::ranked_alphabet, 'b) interp \<Rightarrow> nat \<Rightarrow> 'a wf_trm \<Rightarrow> 'b mem \<Rightarrow> 'b mem"
-  where
-  "wf_assign D x s mem = set_mem x (eval_wf_trm D mem s) mem"
-
-lemma wf_assign_is_assign: "s \<in> trms \<Longrightarrow> wf_assign D x (Abs_wf_trm s) mem = assign D x s mem"
-  by (metis Abs_wf_trm_inverse assign_def eval_wf_trm_def wf_assign_def)
-
 lemma eval_assign1:
-  assumes xy: "x \<noteq> y" and ys: "y \<notin> FV' s"
+  assumes xy: "x \<noteq> y" and ys: "y \<notin> FV s"
   shows "assign D y t (assign D x s mem) = assign D x s (assign D y (trm_subst x s t) mem)"
   apply (induct t rule: trm_simple_induct)
   apply (simp add: assign_def set_mem_def)
@@ -428,14 +480,8 @@ proof
     by (smt eval_trm_eq_mem map_eq_conv xy ys)
 qed
 
-lemma eval_wf_assign1:
-  assumes xy: "x \<noteq> y" and ys: "y \<notin> FV s"
-  shows "wf_assign D y t (wf_assign D x s mem) = wf_assign D x s (wf_assign D y (wf_trm_subst x s t) mem)"
-  apply (insert xy ys, induct s, induct t)
-  by (metis FV_is_FV' Rep_wf_trm_cases Rep_wf_trm_inverse eval_assign1 trm_subst_wf wf_assign_is_assign wf_trm_subst_def)
-
 lemma eval_assign2:
-  assumes xy: "x \<noteq> y" and xs: "x \<notin> FV' s"
+  assumes xy: "x \<noteq> y" and xs: "x \<notin> FV s"
   shows "assign D y t (assign D x s mem) =
          assign D y (trm_subst x s t) (assign D x s mem)"
   apply (induct t rule: trm_simple_induct)
@@ -458,13 +504,6 @@ proof
     by (smt eval_trm_eq_mem map_eq_conv xy xs)
 qed
 
-lemma eval_wf_assign2:
-  assumes xy: "x \<noteq> y" and xs: "x \<notin> FV s"
-  shows "wf_assign D y t (wf_assign D x s mem) =
-         wf_assign D y (wf_trm_subst x s t) (wf_assign D x s mem)"
-  apply (insert xy xs, induct t, induct s)
-  by (metis Abs_wf_trm_inverse FV_is_FV' eval_assign2 trm_subst_wf wf_assign_is_assign wf_trm_subst_def)
-
 lemma eval_assign3: "assign D x t (assign D x s mem) = assign D x (trm_subst x s t) mem"
 proof (induct t rule: trm_simple_induct, simp add: assign_def set_mem_def, auto, default)
   fix f ts v
@@ -478,13 +517,22 @@ proof (induct t rule: trm_simple_induct, simp add: assign_def set_mem_def, auto,
     by (auto simp add: assign_def set_mem_def o_def, smt map_eq_conv)
 qed
 
-lemma eval_wf_assign3:
-  "wf_assign D x t (wf_assign D x s mem) = wf_assign D x (wf_trm_subst x s t) mem"
-  apply (induct t, induct s)
-  by (metis Rep_wf_trm_cases Rep_wf_trm_inverse eval_assign3 trm_subst_wf wf_assign_is_assign wf_trm_subst_def)
-
 lemma eval_halt:
   "x \<notin> output_vars TYPE('a::ranked_alphabet) \<Longrightarrow> halt_null D mem = halt_null D (assign D x (App (NULL::'a) []) mem)"
   by (auto simp add: halt_null_def assign_def set_mem_def)
+
+lemma subst_preds: "P \<in> wf_preds \<Longrightarrow> P[x|s] \<in> wf_preds"
+  apply (induct P)
+  apply simp
+  by (metis SKAT_Term.pred.inject length_map wf_preds.simps)
+
+lemma eval_assign4: "P \<in> preds \<Longrightarrow> eval_pred D (assign D x t mem) P = eval_pred D mem (pred_subst x t P)"
+proof (induct P)
+  fix P and xs :: "'a trm list" assume "Pred P xs \<in> preds"
+  have "\<And>s. s \<in> set xs \<Longrightarrow> eval_trm D (assign D x t mem) s = eval_trm D mem (s[x|t])"
+    by (metis eval_assign3 set_mem_def assign_def)
+  thus "eval_pred D (assign D x t mem) (Pred P xs) = eval_pred D mem (pred_subst x t (Pred P xs))"
+    by (simp add: o_def, metis (lifting) map_ext)
+qed
 
 end
