Carrier/SKAT_Euclid.thy
@@ -1,0 +1,257 @@
+theory SKAT_Euclid
+  imports SKAT_Eval GCD
+begin
+
+datatype alph = mod_alph | plus_alph | nat_alph nat | eq_alph
+
+lemma alph_UNIV: "UNIV = {mod_alph,eq_alph,plus_alph} \<union> (nat_alph ` UNIV)"
+  by (auto simp add: image_def, metis alph.exhaust)
+
+instantiation alph :: ranked_alphabet
+begin
+
+  fun arity_alph :: "alph \<Rightarrow> nat" where
+    "arity_alph mod_alph = 2"
+  | "arity_alph plus_alph = 2"
+  | "arity_alph eq_alph = 2"
+  | "arity_alph is_gcd_alph = 0"
+  | "arity_alph (nat_alph _) = 0"
+
+  definition funs_alph :: "alph set" where "funs_alph \<equiv> {mod_alph,plus_alph} \<union> (nat_alph ` UNIV)"
+
+  definition rels_alph :: "alph set" where "rels_alph \<equiv> {eq_alph}"
+
+  definition NULL_alph :: "alph" where "NULL_alph \<equiv> nat_alph 0"
+
+  declare funs_alph_def [alphabet]
+    and rels_alph_def [alphabet]
+    and NULL_alph_def [alphabet]
+
+  definition output_vars_alph :: "alph itself \<Rightarrow> nat set" where "output_vars_alph x \<equiv> {0}"
+
+  declare output_vars_alph_def [alphabet]
+
+  instance proof
+    show "(funs :: alph set) \<inter> rels = {}"
+      by (auto simp add: funs_alph_def rels_alph_def)
+
+    show "(funs :: alph set) \<union> rels = UNIV"
+      by (auto simp add: funs_alph_def rels_alph_def alph_UNIV)
+
+    show "(funs :: alph set) \<noteq> {}"
+      by (simp add: funs_alph_def)
+
+    show "(rels :: alph set) \<noteq> {}"
+      by (simp add: rels_alph_def)
+
+    show "NULL \<in> (funs :: alph set)"
+      by (simp add: NULL_alph_def funs_alph_def)
+
+    show "arity (NULL::alph) = 0"
+      by (simp add: NULL_alph_def)
+
+    show "\<exists>x. x \<in> output_vars TYPE(alph)"
+      by (metis (mono_tags) insertI1 output_vars_alph_def)
+
+    show "finite (output_vars TYPE(alph))"
+      by (metis (hide_lams, mono_tags) atLeastLessThan0 finite_atLeastLessThan finite_insert output_vars_alph_def)
+  qed
+end
+
+definition MOD :: "alph trm \<Rightarrow> alph trm \<Rightarrow> alph trm" where
+  "MOD a b \<equiv> (App mod_alph [a, b])"
+
+definition PLUS :: "alph trm \<Rightarrow> alph trm \<Rightarrow> alph trm" where
+  "PLUS a b = (App plus_alph [a, b])"
+
+definition EQ :: "alph trm \<Rightarrow> alph trm \<Rightarrow> alph pred" where
+  "EQ x y \<equiv> Pred eq_alph [x, y]"
+
+definition NAT :: "nat \<Rightarrow> alph trm" where
+  "NAT n \<equiv> App (nat_alph n) []"
+
+declare MOD_def [skat_simp]
+  and PLUS_def [skat_simp]
+  and EQ_def [skat_simp]
+  and NAT_def [skat_simp]
+
+fun euclid_funs :: "alph \<Rightarrow> nat list \<Rightarrow> nat" where
+  "euclid_funs mod_alph [x, y] = x mod y"
+| "euclid_funs plus_alph [x, y] = x + y"
+| "euclid_funs (nat_alph n) [] = n"
+| "euclid_funs _ _ = 0"
+
+inductive_set euclid_rels :: "alph \<Rightarrow> nat relation" for a :: "alph" where
+  "a = eq_alph \<Longrightarrow> [x,x] \<in> euclid_rels a"
+
+lemma [simp]: "[x, y] \<in> euclid_rels eq_alph \<longleftrightarrow> x = y"
+  by (metis (lifting) euclid_rels.simps list.inject)
+
+abbreviation EUCLID :: "(alph, nat) interp" where "EUCLID \<equiv> \<lparr>carrier = UNIV, mf = euclid_funs, mr = euclid_rels\<rparr>"
+
+interpretation interp EUCLID done
+
+definition SIMPLE_LOOP :: "alph skat" where
+  "SIMPLE_LOOP \<equiv>
+   WHILE !(pred (EQ (Var 0) (NAT 5))) DO
+     0 := PLUS (Var 0) (NAT 1)
+   WEND"
+
+definition GCD :: "alph skat" where
+  "GCD \<equiv>
+   WHILE !(pred (EQ (Var 1) (NAT 0))) DO
+     2 := Var 1;
+     1 := MOD (Var 0) (Var 1);
+     0 := Var 2
+   WEND"
+
+abbreviation hoare_triple_notation :: "nat mems \<Rightarrow> alph skat \<Rightarrow> nat mems \<Rightarrow> bool" ("_ \<lbrace> _ \<rbrace> _" [54,54,54] 53) where
+  "hoare_triple_notation \<equiv> interp.hoare_triple EUCLID"
+
+abbreviation module_notation :: "nat mems \<Rightarrow> alph skat \<Rightarrow> nat mems" (infix "\<Colon>" 75) where
+  "module_notation \<Delta> x \<equiv> interp.module EUCLID \<Delta> x"
+
+lemma helper: "\<lbrakk>\<And>x. P x = Q x\<rbrakk> \<Longrightarrow> {x. P x} = {x. Q x}"
+  by auto
+
+lemma "P \<lbrace> p \<rbrace> UNIV"
+  by (metis hoare_triple_def top_greatest)
+
+lemma "{} \<lbrace> p \<rbrace> P"
+  by (metis bot_least hoare_triple_def interp.mod_empty)
+
+lemma set_mem_UNIV [simp]: "set_mems x (\<lambda>mem. m) UNIV = {mem. m = mem x}"
+  by (auto simp add: set_mems_def image_def set_mem_def) (rule_tac x = xa in exI, auto)
+
+lemma satisfies_assign: "satisfies x (op = m) = UNIV \<Colon> x := NAT m"
+  by (simp add: satisfies_def module_def NAT_def, transfer, simp add: assigns_def)
+
+lemma skat_assign3_var: "r = t[x|s] \<Longrightarrow> (x := s \<cdot> x := t) = (x := r)"
+  by (metis skat_assign3)
+
+lemma variable_update: "satisfies x (op = n) \<lbrace> x := NAT m \<rbrace> satisfies x (op = m)"
+  apply (simp add: satisfies_assign)
+  apply (rule hoare_assignment'_var)
+  apply (subst mod_mult[symmetric])
+  apply (rule arg_cong) back
+  apply (rule skat_assign3_var[symmetric])
+  by (auto simp add: NAT_def)
+
+  lemma while:
+    assumes b_test: "b \<in> carrier tests"
+    and Q_def: "Q = P \<inter> (UNIV \<Colon> !b)"
+    and loop_condition: "P \<inter> (UNIV \<Colon> b) \<lbrace>p\<rbrace> P"
+    shows "P \<lbrace> WHILE b DO p WEND \<rbrace> Q"
+    by (metis (lifting) Q_def b_test interp.hoare_while loop_condition)
+
+  lemma strengthen_precondition [consumes 1]: "\<lbrakk>P \<lbrace> p \<rbrace> Q; P' \<subseteq> P\<rbrakk> \<Longrightarrow> P' \<lbrace> p \<rbrace> Q"
+    by (metis interp.hoare_weakening order_refl)
+
+lemma [simp]: "satisfies x P \<subseteq> satisfies x Q \<longleftrightarrow> (\<forall>mem. P (mem x) \<longrightarrow> Q (mem x))"
+  by (auto simp add: satisfies_def)
+
+lemma [simp]: "UNIV \<Colon> pred_expr (BLeaf (EQ (Var n) (NAT m))) = satisfies n (op = m)"
+  apply (simp add: module_def EQ_def NAT_def satisfies_def)
+  apply transfer
+  apply auto
+  by (metis empty_iff singleton_iff)
+
+lemma [simp]: "UNIV \<Colon> pred_expr (BNot (BLeaf (EQ (Var n) (NAT m)))) = satisfies n (op \<noteq> m)"
+  apply (simp add: module_def EQ_def NAT_def satisfies_def)
+  apply transfer
+  apply auto
+  by (metis empty_iff singleton_iff)
+
+declare pred_to_expr [simp]
+declare pred_expr_not [simp]
+
+lemma [simp]: "pred_expr (BNot (BNot P)) = pred_expr P"
+  sorry
+
+declare pred_expr_closed [simp]
+
+lemma weakening [consumes 1]: "\<lbrakk>P \<lbrace> p \<rbrace> Q; P' \<subseteq> P; Q \<subseteq> Q'\<rbrakk> \<Longrightarrow> P' \<lbrace> p \<rbrace> Q'"
+  by (metis (lifting) hoare_weakening)
+
+lemma simple_loop_example: "satisfies 0 (op = 0) \<lbrace> SIMPLE_LOOP \<rbrace> satisfies 0 (op = 5)"
+proof -
+  let ?invariant = "satisfies 0 (\<lambda>x. x \<le> 5)"
+
+  have "?invariant \<lbrace> SIMPLE_LOOP \<rbrace> satisfies 0 (op = 5)"
+  proof (simp add: SIMPLE_LOOP_def, rule while, simp_all)
+    show "satisfies 0 (op = 5) = ?invariant \<inter> satisfies 0 (op = 5)"
+      by (auto simp add: satisfies_def)
+
+    have "satisfies 0 (\<lambda>y. y \<le> 4) \<lbrace> 0 := PLUS (Var 0) (NAT (Suc 0)) \<rbrace> satisfies 0 (\<lambda>y. 1 \<le> y \<and> y \<le> 5)"
+      apply (rule hoare_assignment_var)
+      apply (auto simp add: assigns_def PLUS_def NAT_def set_mems_def image_def set_mem_def satisfies_def)
+      apply (rule_tac x = "\<lambda>v. if v = 0 then x 0 - 1 else x v" in exI)
+      by auto
+
+    thus "?invariant \<inter> satisfies 0 (\<lambda>y. y \<noteq> 5)
+            \<lbrace> 0 := PLUS (Var 0) (NAT (Suc 0)) \<rbrace>
+          ?invariant"
+      by (rule weakening, auto simp add: satisfies_def)
+  qed
+
+  thus ?thesis
+    by (rule strengthen_precondition, simp)
+qed
+
+fun initial_mem :: "nat \<Rightarrow> nat \<Rightarrow> nat \<Rightarrow> nat" where
+  "initial_mem x y 0 = x"
+| "initial_mem x y (Suc 0) = y"
+| "initial_mem x y _ = 0"
+
+declare pred_to_expr [simp]
+declare pred_expr_not [simp]
+declare Nat.One_nat_def [simp del]
+
+no_notation
+  dioid.one ("1\<index>") and
+  dioid.zero ("0\<index>")
+
+lemma (in interp) assignment: "P[x|s] \<subseteq> Q \<Longrightarrow> P \<lbrace> x := s \<rbrace> Q"
+  by (metis hoare_triple_def mod_assign)
+
+lemma euclids_algorithm: "{mem. mem 0 = x \<and> mem 1 = y} \<lbrace> GCD \<rbrace> {mem. mem 0 = gcd x y}"
+proof -
+  let ?invariant = "{mem. gcd (mem 0) (mem 1) = gcd x y}"
+
+  have "?invariant \<lbrace> GCD \<rbrace> {mem. mem 0 = gcd x y \<and> mem 1 = 0}"
+  proof (simp add: GCD_def, rule while, simp_all)
+    show "{mem. mem 0 = gcd x y \<and> mem 1 = 0} = ?invariant \<inter> satisfies 1 (op = 0)"
+      by (auto simp add: satisfies_def)
+
+    show "{mem. gcd (mem 0) (mem 1) = gcd x y} \<inter> satisfies 1 (op < 0)
+            \<lbrace> 2 := Var 1 ; 1 := MOD (Var 0) (Var 1) ; 0 := Var 2 \<rbrace>
+          {mem. gcd (mem 0) (mem 1) = gcd x y}"
+    proof (rule hoare_composition)+
+      show "?invariant \<inter> satisfies 1 (op < 0) \<lbrace> 2 := Var 1 \<rbrace> ?invariant \<inter> satisfies 1 (op < 0) \<inter> {mem. mem 1 = mem 2}"
+        apply (rule assignment)
+        by (auto simp add: assigns_def set_mems_def image_def set_mem_def satisfies_def)
+
+      show "?invariant \<inter> satisfies 1 (op < 0) \<inter> {mem. mem 1 = mem 2}
+              \<lbrace> 1 := MOD (Var 0) (Var 1) \<rbrace>
+            {mem. mem 1 = (mem 0) mod (mem 2)} \<inter> {mem. gcd (mem 0) (mem 2) = gcd x y} \<inter> satisfies 2 (op \<noteq> 0)"
+        apply (rule assignment)
+        by (auto simp add: assigns_def set_mems_def image_def set_mem_def satisfies_def MOD_def)
+
+      have "{mem. mem 1 = (mem 0) mod (mem 2)} \<inter> {mem. gcd (mem 0) (mem 2) = gcd x y}
+              \<lbrace> 0 := Var 2 \<rbrace>
+            ?invariant \<inter> {mem. mem 0 = mem 2}"
+        apply (rule assignment)
+        apply (auto simp add: assigns_def set_mems_def image_def set_mem_def satisfies_def)
+        by (metis gcd_red_nat)
+
+      thus "{mem. mem 1 = (mem 0) mod (mem 2)} \<inter> {mem. gcd (mem 0) (mem 2) = gcd x y} \<inter> satisfies 2 (op \<noteq> 0)
+              \<lbrace> 0 := Var 2 \<rbrace>
+            ?invariant"
+        by (rule weakening, auto)
+    qed
+  qed
+  thus ?thesis
+    by (rule weakening, auto)
+qed
+
+end
